src/tls/KDF.Common.fst
@@ -1,0 +1,73 @@
+(*--build-config
+options:--use_hints --fstar_home ../../../FStar --include ../../../FStar/ucontrib/Platform/fst/ --include ../../../FStar/ucontrib/CoreCrypto/fst/ --include ../../../FStar/examples/low-level/crypto/real --include ../../../FStar/examples/low-level/crypto/spartan --include ../../../FStar/examples/low-level/LowCProvider/fst --include ../../../FStar/examples/low-level/crypto --include ../../libs/ffi --include ../../../FStar/ulib/hyperstack --include ideal-flags;
+--*)
+(**
+ Shared state for secret expansion and salt expansion
+ This file exists to break a cyclic module dependency:
+ KDF.Salt.* operates on the same secrets as KDF.Expand
+ but both cannot be implemented in a single module because
+ of the cyclic dependency.
+ *)
+module KDF.Common
+
+open FStar.Heap
+open FStar.HyperHeap
+open FStar.HyperStack
+
+open Platform.Bytes
+open Platform.Error
+open TLSError
+open TLSConstants
+open TLSInfo
+
+module MM = MonotoneMap
+module MR = FStar.Monotonic.RRef
+module HH = FStar.HyperHeap
+module HS = FStar.HyperStack
+
+(* Source index is a secret index *)
+type id = secretId
+
+(* The kind of expansion, either salt of expanded secret *)
+type expand_kind (i:id) =
+  | ExpandSalt: expand_kind i
+  | ExpandSecret:
+     log: hashed_log ->
+     li: logInfo{
+         (EarlySecretID? i ==> LogInfo_CH? li) /\
+         (HandshakeSecretID? i ==> LogInfo_SH? li) /\
+         (ApplicationSecretID? i ==> LogInfo_SF? li) /\
+         log_info li log
+       } ->
+     expand_kind i
+
+// Conceptually, this is either a KDF.Salt.X.state i or KDF.Expand.state i
+// However, the table stores actual key values, and the proper interface for
+// accessing it is spread between KDF.Salt.X and KDF.Expand
+type extracted_secret (#i:id) (x:expand_kind i) =
+  lbytes (Hashing.Spec.tagLen (secretId_hash i))
+
+type expand_log (i:id) (r:rgn) =
+  (if Flags.ideal_KEF then
+    MM.t r (expand_kind i) (extracted_secret #i) (fun _ -> True)
+  else
+    unit)
+
+type state (i:id) =
+  | State:
+    r:rgn ->
+    log: expand_log i r ->
+    state i
+
+let kdf_region:rgn = new_region tls_tables_region
+type kdf_instance_table =
+  (if Flags.ideal_KEF then
+    MM.t kdf_region id state (fun _ -> True)
+  else
+    unit)
+
+let kdf_instances : kdf_instance_table =
+  (if Flags.ideal_KEF then
+    MM.alloc #kdf_region #id #state #(fun _ -> True)
+  else
+    ())
